CAM/NormalForm.v
@@ -1,0 +1,74 @@
+Require Import Lang.NormalForm.
+Require Import Lang.ContextProperties.
+Require Import CAM.Syntax.
+Require Import CAM.Semantics.
+Require Import Tactics.General.
+
+Inductive cam_nf {V : Set} : cam_state V -> Prop :=
+  | cam_nf_val (v : value V) : cam_nf ⟨v, i_ctx_top⟩ₑ
+  | cam_nf_add1 : forall C v1 v2, non_nat v1 -> cam_nf ⟨e_add v1 v2, C⟩ₑ
+  | cam_nf_add2 : forall C v1 v2, non_nat v2 -> cam_nf ⟨e_add v1 v2, C⟩ₑ
+  | cam_nf_app : forall C v1 v2, non_lam v1  -> cam_nf ⟨e_app v1 v2, C⟩ₑ
+  | cam_nf_do : forall C l v, cam_nf ⟨i_ctx_top, C, l, v⟩ₒ.
+
+Lemma HandlesOp_dec :
+  forall {V : Set} (h : handler V) (l : string),
+    HandlesOp h l \/ ~HandlesOp h l.
+Admitted.
+
+Theorem cam_nf_correct :
+  forall (V : Set) (s : cam_state V),
+    cam_nf s <-> normal_form cam_red s.
+Proof.
+  intros. split.
+  (* cam_nf s -> normal_form cam_red s *)
+  - intros H. inv H.
+    + intros [s Hstep]. inv Hstep.
+    + intros [s Hstep]. inv Hstep. inv H0.
+    + intros [s Hstep]. inv Hstep. inv H0.
+    + intros [s Hstep]. inv Hstep. inv H0.
+    + intros [s Hstep]. inv Hstep.
+
+  (* normal_form cam_red s -> cam_nf s  *)
+  - intros H. unfold normal_form in H. destruct s.
+    + destruct e.
+      * destruct C.
+        -- apply cam_nf_val.
+        -- exfalso. apply H. eexists. constructor.
+        -- exfalso. apply H. eexists. constructor.
+      * destruct v1; destruct v2.
+        -- exfalso. apply H. eexists. constructor.
+        -- apply cam_nf_add2. constructor.
+        -- apply cam_nf_add2. constructor.
+        -- apply cam_nf_add1. constructor.
+        -- apply cam_nf_add1. constructor.
+        -- apply cam_nf_add1. constructor.
+        -- apply cam_nf_add1. constructor.
+        -- apply cam_nf_add1. constructor.
+        -- apply cam_nf_add1. constructor.
+      * destruct v1.
+        -- apply cam_nf_app. constructor.
+        -- apply cam_nf_app. constructor.
+        -- exfalso. apply H. eexists. constructor.
+      * exfalso. apply H. eexists. constructor.
+      * exfalso. apply H. eexists. constructor.
+      * exfalso. apply H. eexists. constructor.
+    + destruct C.
+      * apply cam_nf_do.
+      * exfalso. apply H. eexists. constructor.
+      * destruct (HandlesOp_dec h l).
+        -- destruct H0 as [e_op He_op].
+           exfalso. apply H. eexists. apply cam_red_op_handle2. apply He_op.
+        -- exfalso. apply H. eexists. apply cam_red_op_handle1. assumption.
+Qed.
+
+Inductive nf_rel_lang_cam {V : Set} : expr V -> cam_state V -> Prop :=
+  | nf_rel_lang_cam_val (v : value V) : nf_rel_lang_cam v ⟨v, i_ctx_top⟩ₑ
+  | nf_rel_lang_cam_add1 : forall C v1 v2, non_nat v1 ->
+      nf_rel_lang_cam (C [e_add v1 v2]ᵢ) ⟨e_add v1 v2, C⟩ₑ
+  | nf_rel_lang_cam_add2 : forall C v1 v2, non_nat v2 ->
+      nf_rel_lang_cam (C [e_add v1 v2]ᵢ) ⟨e_add v1 v2, C⟩ₑ
+  | nf_rel_lang_cam_app : forall C v1 v2, non_lam v1 ->
+      nf_rel_lang_cam (C [e_app v1 v2]ᵢ) ⟨e_add v1 v2, C⟩ₑ
+  | nf_rel_lang_cam_do : forall C v l, ~IctxHandlesOp C l ->
+      nf_rel_lang_cam (C[ e_do l v ]ᵢ) ⟨i_ctx_top, toₒ C, l, v⟩ₒ.
