Tactics/General.v
@@ -1,0 +1,11 @@
+Require Import Lang.Syntax.
+
+Ltac inv H := inversion H; subst; clear H.
+
+Ltac Handles_contra :=
+  match goal with
+  | [ H1 : ~HandlesOp ?h ?l, H2 : HandlesOpWith ?h ?l ?e  |- _ ] =>
+      let H := fresh "H" in
+      assert (H : HandlesOp h l);
+      [ exists e; assumption | auto ]
+  end.
